Lean4Lean/Expr.lean
@@ -7,20 +7,6 @@ def prop : Expr := .sort .zero
 
 def arrow (d b : Expr) : Expr := .forallE `a d b .default
 
-def realLooseBVarRange : Expr → Nat
-  | .bvar i => i + 1
-  | .const ..
-  | .sort _
-  | .fvar _
-  | .mvar _
-  | .lit _ => 0
-  | .mdata _ e
-  | .proj _ _ e => e.realLooseBVarRange
-  | .app e1 e2 => max e1.realLooseBVarRange e2.realLooseBVarRange
-  | .lam _ e1 e2 _
-  | .forallE _ e1 e2 _ => max e1.realLooseBVarRange (e2.realLooseBVarRange - 1)
-  | .letE _ e1 e2 e3 _ => max (max e1.realLooseBVarRange e2.realLooseBVarRange) (e3.realLooseBVarRange - 1)
-
 namespace ReplaceImpl
 
 unsafe abbrev ReplaceT := StateT (PtrMap Expr Expr)
